DS/BST2.v
@@ -1,0 +1,291 @@
+Require Export RCCBase.
+Require Import Data.BTree.
+Require Import Ord.
+Require Import Sorting.Sort.
+
+(** * Definitions of the bst property. *)
+
+Inductive isBST2
+  {A : Type} {cmp : A -> A -> comparison} : BTree A -> Prop :=
+    | isBST2_empty : isBST2 empty
+    | isBST2_node :
+        forall (v : A) (l r : BTree A),
+          All (fun x : A => cmp x v = Lt) l ->
+          All (fun x : A => cmp x v = Gt) r ->
+            isBST2 l -> isBST2 r -> isBST2 (node v l r).
+
+Arguments isBST2 {A} _ _.
+
+Hint Constructors All isBST2 : core.
+
+Ltac isBST2 :=
+repeat match goal with
+    |                          |- isBST2 _ empty  => constructor
+    |                          |- isBST2 _ _ -> _ => intro
+    | H : isBST2 _ empty        |- _              => clear H
+    | H : isBST2 _ (node _ _ _) |- _              => inv H
+end; auto.
+
+Ltac isBST2' :=
+repeat match goal with
+    |                           |- isBST2 _ _      => constructor; auto
+    |                           |- isBST2 _ _ -> _ => intro
+    | H : isBST2 _ empty        |- _               => clear H
+    | H : isBST2 _ (node _ _ _) |- _               => inv H
+end; auto.
+
+(** * BST functions *)
+
+Fixpoint partition
+  {A : Type} (cmp : A -> A -> comparison) (x : A) (t : BTree A)
+  : BTree A * bool * BTree A :=
+match t with
+    | empty      => (empty, false, empty)
+    | node v l r =>
+        match cmp x v with
+            | Lt =>
+                match partition cmp x l with
+                    | (l1, b, l2) => (l1, b, node v l2 r)
+                end
+            | Eq => (l, true, r)
+            | Gt =>
+                match partition cmp x r with
+                    | (r1, b, r2) => (node v l r1, b, r2)
+                end
+        end
+end.
+
+Functional Scheme partition_ind := Induction for partition Sort Prop.
+
+Function union {A : Type} (cmp : A -> A -> comparison) (t1 t2 : BTree A) : BTree A :=
+match t1 with
+    | empty => t2
+    | node v1 l1 r1 =>
+        match partition cmp v1 t2 with
+            | (l, _, r) => node v1 (union cmp l1 l) (union cmp r1 r)
+        end
+end.
+
+Function intersection {A : Type} (cmp : A -> A -> comparison) (t1 t2 : BTree A) : BTree A :=
+match t1 with
+    | empty => empty
+    | node v1 l1 r1 =>
+        match partition cmp v1 t2 with
+            | (l, b, r)  =>
+                let l' := intersection cmp l1 l in
+                let r' := intersection cmp r1 r in
+                  if b
+                  then node v1 l' r'
+                  else union cmp l' r'
+        end
+end.
+
+Function difference {A : Type} (cmp : A -> A -> comparison) (t1 t2 : BTree A) : BTree A :=
+match t1 with
+    | empty => empty
+    | node v1 l1 r1 =>
+        let '(l, b, r) := partition cmp v1 t2 in
+        let l' := difference cmp l1 l in
+        let r' := difference cmp r1 r in
+          if b
+          then union cmp l' r'
+          else
+            node v1 l' r'
+end.
+
+Definition insert
+  {A : Type} (cmp : A -> A -> comparison)
+  (x : A) (t : BTree A) : BTree A :=
+    union cmp (singleton x) t.
+
+Definition remove
+  {A : Type} (cmp : A -> A -> comparison)
+  (x : A) (t : BTree A) : BTree A :=
+    difference cmp t (singleton x).
+
+Definition test : BTree nat :=
+  node 50
+    (node 25
+      (node 10 empty empty)
+      (node 40 empty empty))
+    (node 75
+      (node 60 empty empty)
+      (node 100 empty empty)).
+
+Definition test' : BTree nat :=
+  node 100
+    (node 75
+      (node 60
+        (node 25
+          (node 10 empty empty)
+          (node 40 empty empty))
+        empty)
+      empty)
+    empty.
+
+Compute union Nat.compare test test'.
+Compute intersection Nat.compare test test'.
+Compute difference Nat.compare test test'.
+Compute insert Nat.compare 123 test.
+Compute remove Nat.compare 50 test.
+
+(** * Properties of partition *)
+
+Lemma partition_spec :
+  forall {A : Ord} {v : A} {t t1 t2 : BTree A} {b : bool},
+    partition cmp v t = (t1, b, t2) ->
+      isBST2 cmp t ->
+        All (fun x : A => cmp x v = Lt) t1 /\
+        All (fun x : A => cmp x v = Gt) t2.
+Proof.
+  intros until t.
+  functional induction partition cmp v t;
+  inv 1; isBST2.
+    trich.
+    edestruct IHp; eauto. repeat constructor; auto.
+      trich.
+      induction H4; constructor; isBST2. trich.
+    edestruct IHp; eauto. split; repeat constructor; auto.
+      trich.
+      induction H3; constructor; isBST2. trich.
+Qed.
+
+Lemma All_partition :
+  forall {A : Type} {P : A -> Prop} {cmp : A -> A -> comparison} {v : A} {t l r : BTree A} {b : bool},
+    partition cmp v t = (l, b, r) ->
+      All P t -> All P l /\ All P r.
+Proof.
+  intros until t.
+  functional induction partition cmp v t;
+  inv 1; inv 1; edestruct IHp; eauto.
+Qed.
+
+Lemma isBST2_partition :
+  forall {A : Type} {cmp : A -> A -> comparison} {v : A} {t l r : BTree A} {b : bool},
+    partition cmp v t = (l, b, r) ->
+      isBST2 cmp t -> isBST2 cmp l /\ isBST2 cmp r.
+Proof.
+  intros until t.
+  functional induction partition cmp v t;
+  inv 1; isBST2.
+    destruct (All_partition e1 H3). edestruct IHp; eauto.
+    destruct (All_partition e1 H4). edestruct IHp; eauto.
+Qed.
+
+Lemma All_union :
+  forall {A : Ord} {P : A -> Prop} {cmp : A -> A -> comparison} {t1 t2 : BTree A},
+    All P t1 -> All P t2 -> All P (union cmp t1 t2).
+Proof.
+  intros until t2.
+  functional induction union cmp t1 t2;
+  inv 1.
+  intro. destruct (All_partition e0 H). constructor; auto.
+Qed.
+
+Lemma isBST2_union :
+  forall {A : Ord} (t1 t2 : BTree A),
+    isBST2 cmp t1 -> isBST2 cmp t2 -> isBST2 cmp (union cmp t1 t2).
+Proof.
+  intros until t2.
+  functional induction union cmp t1 t2;
+  isBST2.
+  {
+    destruct (isBST2_partition e0 H0).
+    destruct (partition_spec e0); auto.
+    isBST2'; apply All_union; auto.
+  }
+Qed.
+
+Lemma All_intersection :
+  forall {A : Ord} {P : A -> Prop} {t1 t2 : BTree A},
+    isBST2 cmp t2 ->
+      All P t1 -> All P t2 ->
+        All P (intersection cmp t1 t2).
+Proof.
+  intros until t2.
+  functional induction intersection cmp t1 t2;
+  inv 2; intro.
+    destruct (isBST2_partition e0), (partition_spec e0); auto. constructor.
+      assumption.
+      apply IHb; auto. admit.
+      apply IHb0; auto. admit.
+    destruct (isBST2_partition e0), (partition_spec e0); auto. apply All_union.
+      apply IHb; auto. admit.
+      apply IHb0; auto. admit.
+Admitted.
+
+Lemma All_intersection_Lt :
+  forall {A : Ord} {P : A -> Prop} {t1 t2 : BTree A} {v : A},
+    isBST2 cmp t2 ->
+      All (fun x : A => cmp x v = Lt) t1 ->
+      All (fun x : A => cmp x v = Lt) t2 ->
+        All (fun x : A => cmp x v = Lt) (intersection cmp t1 t2).
+Proof.
+  intros until t2.
+  functional induction intersection cmp t1 t2;
+  inv 2; intro.
+    destruct (isBST2_partition e0), (partition_spec e0); auto. constructor.
+      assumption.
+      apply IHb; auto. clear e0 IHb IHb0. induction H3; constructor; isBST2; trich.
+      admit.
+    destruct (isBST2_partition e0), (partition_spec e0); auto. apply All_union.
+      apply IHb; auto. clear e0 IHb IHb0. induction H3; constructor; isBST2; trich.
+      clear IHb IHb0. induction H0; inv e0; isBST2; intros.
+        admit.
+        trich.
+          destruct (partition cmp v1 l), p; inv H9.
+Admitted.
+
+Lemma isBST_intersection :
+  forall {A : Ord} {t1 t2 : BTree A},
+    isBST2 cmp t1 -> isBST2 cmp t2 ->
+      isBST2 cmp (intersection cmp t1 t2).
+Proof.
+  intros until t2.
+  functional induction intersection cmp t1 t2;
+  isBST2.
+    destruct (isBST2_partition e0), (partition_spec e0); auto. constructor.
+      apply All_intersection; auto.
+      apply All_intersection; auto.
+      apply IHb; auto.
+      apply IHb0; auto.
+    destruct (isBST2_partition e0); auto. apply isBST2_union.
+      apply IHb; auto.
+      apply IHb0; auto.
+Qed.
+
+Lemma All_difference :
+  forall {A : Ord} {P : A -> Prop} {t1 t2 : BTree A},
+    isBST2 cmp t2 ->
+      All P t1 -> All P t2 ->
+        All P (difference cmp t1 t2).
+Proof.
+  intros until t2.
+  functional induction difference cmp t1 t2;
+  inv 2; intro.
+    destruct (isBST2_partition e0), (partition_spec e0); auto. apply All_union.
+      apply IHb; auto. admit.
+      apply IHb0; auto. admit.
+    destruct (isBST2_partition e0), (partition_spec e0); auto. constructor.
+      assumption.
+      apply IHb; auto. admit.
+      apply IHb0; auto. admit.
+Admitted.
+
+Lemma isBST2_difference :
+  forall {A : Ord} {t1 t2 : BTree A},
+    isBST2 cmp t1 -> isBST2 cmp t2 ->
+      isBST2 cmp (difference cmp t1 t2).
+Proof.
+  intros until t2.
+  functional induction difference cmp t1 t2;
+  isBST2.
+    destruct (isBST2_partition e0); auto. apply isBST2_union.
+      apply IHb; auto.
+      apply IHb0; auto.
+    destruct (isBST2_partition e0), (partition_spec e0); auto. constructor.
+      apply All_difference; auto.
+      apply All_difference; auto.
+      apply IHb; auto.
+      apply IHb0; auto.
+Qed.
